coq/coq2ml.v
@@ -1,0 +1,63 @@
+Require Import String.
+
+Require Import foltl.
+Require Import api.
+Require Import dec.
+Require Import finite.
+Require utils.
+
+Section COQ2ML.
+
+  Context {Ts: Type} {Tv: Ts->Type} {Tc: Ts->Type} {Tp: Type}.
+  Variable Sg: @Sig Ts Tv Tc Tp.
+
+  Variable sort2ml: Sort (Sig:=Sg) -> mlSort.
+  Variable varName : forall {s: Sort (Sig:=Sg)}, variable (Sig:=Sg) s -> string.
+  Variable cstName : forall {s: Sort (Sig:=Sg)}, constant (Sig:=Sg) s -> string.
+  Variable relName : predicate (Sig:=Sg) -> string.
+
+  Definition var2ml {s: Sort (Sig:=Sg)} (v: variable (Sig:=Sg) s) : mlVariable := {|
+    mlVarName := varName v;
+    mlVarSort := sort2ml s;
+  |}.
+
+  Definition cst2ml {s: Sort (Sig:=Sg)} (c: constant (Sig:=Sg) s) : mlConstant := {|
+    mlCstName := cstName c;
+    mlCstSort := sort2ml s;
+  |}.
+
+  Definition rel2ml (r: predicate (Sig:=Sg)) : string := relName r.
+
+  Definition tm2ml {s} (tm: term Sg s) :=
+    match tm with
+      Var _ _ v => MLVar (var2ml v)
+    | Cst _ _ c => MLCst (cst2ml c)
+    end.
+
+  Definition lt2ml (l: literal Sg) :=
+    match l with
+      PApp _ x p a => MLPApp x (rel2ml p) (utils.fmap (fun i => tm2ml (a i)))
+    end.
+
+  Definition at2ml (a: atom Sg) :=
+  match a with
+    Literal _ l => MLLiteral (lt2ml l)
+  | NLiteral _ l => MLNLiteral (lt2ml l)
+  | Eq _ s t1 t2 => MLEq (tm2ml t1) (tm2ml t2)
+  | NEq _ s t1 t2 => MLNEq (tm2ml t1) (tm2ml t2)
+  end.
+
+  Fixpoint fm2ml (f: formula Sg) :=
+  match f with
+    | FTrue _ => MLFTrue
+    | FFalse _ => MLFFalse
+    | Atom _ a => MLAtom (at2ml a)
+    | And _ f1 f2 => MLAnd (fm2ml f1) (fm2ml f2)
+    | Or _ f1 f2 => MLOr (fm2ml f1) (fm2ml f2)
+    | Ex _ s v f => MLEx (var2ml v) (fm2ml f)
+    | All _ s v f => MLAll (var2ml v) (fm2ml f)
+    | F _ f => MLF(fm2ml f)
+    | G _ f => MLG (fm2ml f)
+  end.
+
+End COQ2ML.
