coq/mlUtils.v
@@ -1,0 +1,578 @@
+Require Import List.
+Require Import String.
+
+Require Import utils.
+
+Require Import api.
+
+Definition mlVarIds v := MLV v :: MLS (mlVarSort v) :: nil.
+
+Definition mlCstIds c := MLC c :: MLS (mlCstSort c) :: nil.
+
+Definition mlRelIds r := MLR r :: (List.map MLS (mlRelArity r)).
+
+Definition mlTermIds tm: list mlIdent :=
+  match tm with
+   MLVar v => mlVarIds v
+  | MLCst c => mlCstIds c
+  end.
+
+Definition mlLitIds l : list mlIdent :=
+  match l with
+    MLPApp nx r args => 
+      mlRelIds {| mlRelName := r; mlRelArity := List.map mlTermSort args |} ++
+        List.concat (List.map mlTermIds args)
+  end.
+
+Definition mlAtomIds a : list mlIdent :=
+  match a with
+  | MLLiteral l => mlLitIds l
+  | MLNLiteral l => mlLitIds l
+  | MLEq t1 t2 => mlTermIds t1 ++ mlTermIds t2
+  | MLNEq t1 t2 => mlTermIds t1 ++ mlTermIds t2
+  end.
+
+Fixpoint mlFormulaIds f :=
+  match f with
+    MLFTrue | MLFFalse => nil
+  | MLAtom a => mlAtomIds a
+  | MLAnd f1 f2 | MLOr f1 f2 => mlFormulaIds f1 ++ mlFormulaIds f2
+  | MLEx v f' | MLAll v f' => MLS (mlVarSort v) :: MLV v :: mlFormulaIds f'
+  | MLF f' | MLG f' => mlFormulaIds f'
+  end.
+
+Definition mlEventIds ev :=
+  List.map MLV (mlEvArgs ev) ++ 
+  List.map MLS (List.map mlVarSort (mlEvArgs ev)) ++
+  mlFormulaIds (mlEvBody ev).
+
+Definition mlPathIds p := mlRelIds (mlTC p) ++ mlRelIds (mlBase p).
+
+Definition mlUsingIds u evts :=
+  match u with
+    TEA => nil
+  | TTC r v f => (mlRelIds r) ++ (mlVarIds v) ++ (mlFormulaIds f)
+  | TFC ef => List.concat (List.map (fun e => mlFormulaIds (ef e)) evts) 
+  end.
+
+Definition mlCheckIds chk evts :=
+  mlFormulaIds (mlChkBody chk) ++
+  mlFormulaIds (mlChkAssumes chk) ++
+  mlUsingIds (mlChkUsing chk) evts.
+
+Definition mlModelIds m :=
+  List.concat (List.map mlFormulaIds (mlAxioms m)) ++
+  List.concat (List.map mlEventIds (mlEvents m)) ++
+  List.concat (List.map mlPathIds (mlClosures m)) ++
+  (mlCheckIds (mlCheckWith m) (mlEvents m)).
+
+Definition mlSorts m := 
+  imap_filter isMLSortDec
+    (mlModelIds m)
+    (fun v h1 h2 => getMLSort v h1).
+
+Definition mlAllVariables m: list mlVariable :=
+  imap_filter isMLVarDec
+    (mlModelIds m)
+    (fun v h1 h2 => getMLVar v h1).
+
+Definition mlVariables m s :=
+  List.filter (fun v => if string_dec (mlVarSort v) s then true else false) (mlAllVariables m).
+
+Definition mlAllConstants m: list mlConstant :=
+  imap_filter isMLCstDec
+    (mlModelIds m)
+    (fun v h1 h2 => getMLCst v h1).
+
+Definition mlConstants m s :=
+  List.filter (fun v => if string_dec (mlCstSort v) s then true else false) (mlAllConstants m).
+
+Definition mlRelations m: list mlRelation :=
+  imap_filter isMLRelDec
+    (mlModelIds m)
+    (fun v h1 h2 => getMLRel v h1).
+
+Lemma mlSortOfTermVarIn:
+ forall v tm, In (MLV v) (mlTermIds tm) -> In (MLS (mlVarSort v)) (mlTermIds tm).
+Proof.
+  intros.
+  destruct tm; simpl in *.
+  destruct H.
+  injection H; intros; subst v0; tauto.
+  destruct H; auto; discriminate.
+
+  destruct H; auto; try discriminate.
+  destruct H; auto; try discriminate.
+Qed.
+
+Lemma mlSortOfTermCstIn:
+ forall c tm, In (MLC c) (mlTermIds tm) -> In (MLS (mlCstSort c)) (mlTermIds tm).
+Proof.
+  intros.
+  destruct tm; simpl in *.
+  destruct H; auto; try discriminate.
+  destruct H; auto; try discriminate.
+
+  destruct H.
+  injection H; intros; subst c0; tauto.
+  destruct H; auto; discriminate.
+Qed.
+
+Lemma mlSortOfLitVarIn:
+ forall v lt, In (MLV v) (mlLitIds lt) -> In (MLS (mlVarSort v)) (mlLitIds lt).
+Proof.
+  intros; destruct lt; simpl in *; intros; auto.
+  destruct H; [left | right]; auto; try discriminate.
+  revert H; apply In_app_imp_In_app; intros.
+  exfalso; revert H; generalize (map mlTermSort args); simpl; intros; auto.
+  apply in_map_iff in H; destruct H as [x [h1 h2]]; subst; auto; discriminate.
+  revert H; apply In_cmap_In_cmap.
+  apply mlSortOfTermVarIn.
+Qed.
+
+Lemma mlSortOfLitCstIn:
+ forall c lt, In (MLC c) (mlLitIds lt) -> In (MLS (mlCstSort c)) (mlLitIds lt).
+Proof.
+  intros; destruct lt; simpl in *; intros; auto.
+  destruct H; [left | right]; auto; try discriminate.
+  revert H; apply In_app_imp_In_app; intros.
+  exfalso; revert H; generalize (map mlTermSort args); simpl; intros; auto.
+  apply in_map_iff in H; destruct H as [x [h1 h2]]; subst; auto; discriminate.
+  revert H; apply In_cmap_In_cmap.
+  apply mlSortOfTermCstIn.
+Qed.
+
+Lemma mlSortOfAtmVarIn:
+ forall v a, In (MLV v) (mlAtomIds a) -> In (MLS (mlVarSort v)) (mlAtomIds a).
+Proof.
+  intros v a; destruct a; simpl; intros.
+  revert H; apply mlSortOfLitVarIn.
+  revert H; apply mlSortOfLitVarIn.
+  revert H; apply In_app_imp_In_app; apply mlSortOfTermVarIn.
+  revert H; apply In_app_imp_In_app; apply mlSortOfTermVarIn.
+Qed.
+
+Lemma mlSortOfAtmCstIn:
+ forall c a, In (MLC c) (mlAtomIds a) -> In (MLS (mlCstSort c)) (mlAtomIds a).
+Proof.
+  intros v a; destruct a; simpl; intros.
+  revert H; apply mlSortOfLitCstIn.
+  revert H; apply mlSortOfLitCstIn.
+  revert H; apply In_app_imp_In_app; apply mlSortOfTermCstIn.
+  revert H; apply In_app_imp_In_app; apply mlSortOfTermCstIn.
+Qed.
+
+Lemma mlSortOfFormVarIn:
+ forall v f, In (MLV v) (mlFormulaIds f) -> In (MLS (mlVarSort v)) (mlFormulaIds f).
+Proof.
+  induction f; simpl; intros; auto.
+  revert H; apply mlSortOfAtmVarIn.
+  revert H; apply In_app_imp_In_app; auto.
+  revert H; apply In_app_imp_In_app; auto.
+
+  destruct H; try discriminate.
+  destruct H.
+  injection H; intros; subst m; tauto.
+  right; right; now auto.
+
+  destruct H; try discriminate.
+  destruct H.
+  injection H; intros; subst m; tauto.
+  right; right; now auto.  
+Qed.
+
+Lemma mlSortOfFormCstIn:
+ forall c f, In (MLC c) (mlFormulaIds f) -> In (MLS (mlCstSort c)) (mlFormulaIds f).
+Proof.
+  induction f; simpl; intros; auto.
+  revert H; apply mlSortOfAtmCstIn.
+  revert H; apply In_app_imp_In_app; auto.
+  revert H; apply In_app_imp_In_app; auto.
+
+  destruct H; try discriminate.
+  destruct H; try discriminate.
+  tauto.
+
+  destruct H; try discriminate.
+  destruct H; try discriminate.
+  tauto.
+Qed.
+
+Lemma mlSortOfTermRelIn: forall tm r s,
+  In s (mlRelArity r) -> In (MLR r) (mlTermIds tm) -> In (MLS s) (mlTermIds tm).
+Proof.
+  intros.
+  destruct tm; simpl in *.
+  destruct H0; try discriminate.
+  destruct H0; try discriminate; tauto.
+  destruct H0; try discriminate.
+  destruct H0; try discriminate; tauto.
+Qed.
+
+Lemma mlSortOfRelRelIn: forall r1 r2 s,
+  In s (mlRelArity r1) -> In (MLR r1) (mlRelIds r2) -> In (MLS s) (mlRelIds r2).
+Proof.
+  intros.
+  unfold mlRelIds in *.
+  destruct H0.
+  injection H0; clear H0; intros; subst r2; simpl.
+  right; apply in_map_iff; exists s; tauto.
+  apply in_map_iff in H0.
+  destruct H0 as [s' [H0 _]]; discriminate.
+Qed.
+
+Lemma mlSortOfLitRelIn: forall lt r s,
+  In s (mlRelArity r) -> In (MLR r) (mlLitIds lt) -> In (MLS s) (mlLitIds lt).
+Proof.
+  intros.
+  destruct lt; simpl in *.
+  destruct H0.
+  injection H0; clear H0; intros; subst r; simpl in *.
+  right.
+  apply in_app_iff.
+  left.
+  apply in_map_iff in H.
+  destruct H as [x [h1 h2]]; subst.
+  apply in_map_iff.
+  exists (mlTermSort x); split; auto.
+  apply in_map_iff.
+  exists x; split; auto.
+  
+  apply in_app_iff in H0.
+  destruct H0.
+  apply in_map_iff in H0.
+  destruct H0 as [x [H0 _]]; discriminate.
+  apply in_concat in H0.
+  destruct H0 as [x [H0 H1]].
+  apply in_map_iff in H0.
+  destruct H0 as [t [h1 h2]]; subst.
+  destruct t; simpl in *.
+  destruct H1; try discriminate.
+  destruct H0; try discriminate; tauto.
+  destruct H1; try discriminate.
+  destruct H0; try discriminate; tauto.
+Qed.
+
+Lemma mlSortOfAtmRelIn: forall a r s,
+  In s (mlRelArity r) -> In (MLR r) (mlAtomIds a) -> In (MLS s) (mlAtomIds a).
+Proof.
+  intros.
+  destruct a; simpl in *; intros; auto.
+  revert H H0; apply mlSortOfLitRelIn.
+  revert H H0; apply mlSortOfLitRelIn.
+  revert H0; apply In_app_imp_In_app; apply mlSortOfTermRelIn; auto.
+  revert H0; apply In_app_imp_In_app; apply mlSortOfTermRelIn; auto.
+Qed.
+
+Lemma mlSortOfFormRelIn: forall f r s,
+  In s (mlRelArity r) -> In (MLR r) (mlFormulaIds f) -> In (MLS s) (mlFormulaIds f).
+Proof.
+  intros.
+  induction f; simpl in *; intros; auto.
+  revert H0; apply mlSortOfAtmRelIn; auto.
+  revert H0; apply In_app_imp_In_app; now auto.
+  revert H0; apply In_app_imp_In_app; now auto.
+  destruct H0; try discriminate; destruct H0; try discriminate; tauto.
+  destruct H0; try discriminate; destruct H0; try discriminate; tauto.
+Qed.
+
+Lemma mlSortOfEvtVarIn:
+  forall v e, In (MLV v) (mlEventIds e) -> In (MLS (mlVarSort v)) (mlEventIds e).
+Proof.
+  unfold mlEventIds; intros.
+  apply in_app_iff in H; destruct H.
+  apply in_map_iff in H.
+  destruct H as [x [h1 h2]].
+  injection h1; clear h1; intros; subst x.
+  apply in_app_iff; right.
+  apply in_app_iff; left.
+  apply in_map_iff.
+  exists (mlVarSort v); split; auto.
+  apply in_map_iff; exists v; now auto.
+  
+  apply in_app_iff in H; destruct H.
+  
+  apply in_map_iff in H.
+  destruct H as [x [H _]]; discriminate.
+  
+  apply in_app_iff; right.
+  
+  apply in_app_iff; right.
+  revert H; apply mlSortOfFormVarIn.
+Qed.
+
+Lemma mlSortOfEvtCstIn:
+  forall c e, In (MLC c) (mlEventIds e) -> In (MLS (mlCstSort c)) (mlEventIds e).
+Proof.
+  unfold mlEventIds; intros.
+  apply in_app_iff in H; destruct H.
+  apply in_map_iff in H.
+  destruct H as [x [H _]]; discriminate.
+  apply in_app_iff in H; destruct H.
+  apply in_map_iff in H.
+  destruct H as [x [H _]]; discriminate.
+  
+  apply in_app_iff; right.
+  apply in_app_iff; right.
+  revert H; apply mlSortOfFormCstIn.
+Qed.
+
+Lemma mlSortOfPathVarIn:
+  forall v p, In (MLV v) (mlPathIds p) -> In (MLS (mlVarSort v)) (mlPathIds p).
+Proof.
+  unfold mlPathIds; intros.
+  revert H; apply In_app_imp_In_app; intros.
+  unfold mlRelIds in H.
+  destruct H; try discriminate.
+  apply in_map_iff in H.
+  destruct H as [x [H _]]; discriminate.
+
+  unfold mlRelIds in H.
+  destruct H; try discriminate.
+  apply in_map_iff in H.
+  destruct H as [x [H _]]; discriminate.
+Qed.
+
+Lemma mlSortOfPathCstIn:
+  forall c p, In (MLC c) (mlPathIds p) -> In (MLS (mlCstSort c)) (mlPathIds p).
+Proof.
+  unfold mlPathIds; intros.
+  revert H; apply In_app_imp_In_app; intros.
+  unfold mlRelIds in H.
+  destruct H; try discriminate.
+  apply in_map_iff in H.
+  destruct H as [x [H _]]; discriminate.
+
+  unfold mlRelIds in H.
+  destruct H; try discriminate.
+  apply in_map_iff in H.
+  destruct H as [x [H _]]; discriminate.
+Qed.
+
+Lemma mlSortOfChkVarIn: forall v m,
+  In (MLV v) (mlCheckIds (mlCheckWith m) (mlEvents m)) ->
+  In (MLS (mlVarSort v)) (mlCheckIds (mlCheckWith m) (mlEvents m)).
+Proof.
+  unfold mlCheckIds; intros.
+  revert H; apply In_app_imp_In_app.
+  apply mlSortOfFormVarIn.
+  apply In_app_imp_In_app.
+  apply mlSortOfFormVarIn.
+  generalize (mlChkUsing (mlCheckWith m)); intro u.
+  unfold mlUsingIds.
+  destruct u; simpl in *; intros; auto.
+  destruct H; try discriminate.
+  right.
+  revert H; apply In_app_imp_In_app.
+  intro.
+  apply in_map_iff in H.
+  destruct H as [x [H _]]; discriminate.
+  intro.
+  destruct H.
+  injection H; clear H; intros; subst m1; simpl; tauto.
+  destruct H; try discriminate.
+  right; right; revert H; apply mlSortOfFormVarIn.
+  revert H; apply In_cmap_In_cmap.
+  intro; apply mlSortOfFormVarIn.
+Qed.
+
+Lemma mlSortOfChkCstIn: forall c m,
+  In (MLC c) (mlCheckIds (mlCheckWith m) (mlEvents m)) ->
+  In (MLS (mlCstSort c)) (mlCheckIds (mlCheckWith m) (mlEvents m)).
+Proof.
+  unfold mlCheckIds; intros.
+  revert H; apply In_app_imp_In_app.
+  apply mlSortOfFormCstIn.
+  apply In_app_imp_In_app.
+  apply mlSortOfFormCstIn.
+  generalize (mlChkUsing (mlCheckWith m)); intro u.
+  unfold mlUsingIds.
+  destruct u; simpl in *; intros; auto.
+  destruct H; try discriminate.
+  right.
+  revert H; apply In_app_imp_In_app.
+  intro.
+  apply in_map_iff in H.
+  destruct H as [x [H _]]; discriminate.
+  intro.
+  destruct H; try discriminate.
+  destruct H; try discriminate.
+  right; right; revert H; apply mlSortOfFormCstIn.
+  revert H; apply In_cmap_In_cmap.
+  intro; apply mlSortOfFormCstIn.
+Qed.
+
+Lemma mlSortOfVarIn: forall m v,
+  In (MLV v) (mlModelIds m) -> In (MLS (mlVarSort v)) (mlModelIds m).
+Proof.
+  intros.
+  unfold mlModelIds in *.
+  revert H.
+  apply utils.In_app_imp_In_app.
+  apply In_cmap_In_cmap.
+  apply mlSortOfFormVarIn.
+
+  apply utils.In_app_imp_In_app.
+  apply In_cmap_In_cmap.
+  apply mlSortOfEvtVarIn.
+
+  apply utils.In_app_imp_In_app.
+  apply In_cmap_In_cmap.
+  apply mlSortOfPathVarIn.
+  
+  apply mlSortOfChkVarIn.
+Qed.
+
+Lemma mlSortOfCstIn: forall m c,
+  In (MLC c) (mlModelIds m) -> In (MLS (mlCstSort c)) (mlModelIds m).
+Proof.
+  intros.
+  unfold mlModelIds in *.
+  revert H.
+  apply utils.In_app_imp_In_app.
+  apply In_cmap_In_cmap.
+  apply mlSortOfFormCstIn.
+
+  apply utils.In_app_imp_In_app.
+  apply In_cmap_In_cmap.
+  apply mlSortOfEvtCstIn.
+
+  apply utils.In_app_imp_In_app.
+  apply In_cmap_In_cmap.
+  apply mlSortOfPathCstIn.
+  
+  apply mlSortOfChkCstIn.
+Qed.
+
+Lemma mlSortOfEvtArityIn: forall e r s, 
+  In s (mlRelArity r) -> In (MLR r) (mlEventIds e) -> In (MLS s) (mlEventIds e).
+Proof.
+  intros.
+  unfold mlEventIds in *.
+  revert H0; apply In_app_imp_In_app.
+  intros.
+  apply in_map_iff in H0.
+  destruct H0 as [v [H0 _]]; discriminate.
+  apply In_app_imp_In_app.
+  intro.
+  apply in_map_iff in H0.
+  destruct H0 as [s' [h1 h2]]; try discriminate.
+  apply mlSortOfFormRelIn; auto.
+Qed.
+
+Lemma mlSortOfPathArityIn: forall p r s,
+  In s (mlRelArity r) -> In (MLR r) (mlPathIds p) -> In (MLS s) (mlPathIds p).
+Proof.
+  intros.
+  unfold mlPathIds in *.
+  revert H0; apply In_app_imp_In_app; simpl; intros.
+  destruct H0.
+  injection H0; clear H0; intros; subst.
+  right.
+  apply in_map_iff; exists s; tauto. 
+  apply in_map_iff in H0.
+  destruct H0 as [s' [h1 _]]; discriminate.
+
+  destruct H0.
+  injection H0; clear H0; intros; subst.
+  right.
+  apply in_map_iff; exists s; tauto. 
+  apply in_map_iff in H0.
+  destruct H0 as [s' [h1 _]]; discriminate.  
+Qed.
+
+Lemma mlSortOfRelUsingArityIn: forall m u r s,
+  In s (mlRelArity r) -> In (MLR r) (mlUsingIds u (mlEvents m)) ->
+    In (MLS s) (mlUsingIds u (mlEvents m)).
+Proof.
+  intros.
+  unfold mlUsingIds in *.
+  destruct u.
+  destruct H0.
+  revert H0; apply In_app_imp_In_app.
+  apply mlSortOfRelRelIn; now auto.
+  apply In_app_imp_In_app.
+  unfold mlVarIds; intro.
+  simpl in H0.
+  destruct H0; try discriminate.
+  destruct H0; try tauto; discriminate.
+  apply mlSortOfFormRelIn; now auto.
+  revert H0; apply In_cmap_In_cmap; intro e.
+  apply mlSortOfFormRelIn; auto.
+Qed.
+
+Lemma mlSortOfRelChkArityIn: forall m r s,
+  In s (mlRelArity r) -> In (MLR r) (mlCheckIds (mlCheckWith m) (mlEvents m))
+   -> In (MLS s) (mlCheckIds (mlCheckWith m) (mlEvents m)).
+Proof.
+  intros.
+  unfold mlCheckIds in *.
+  revert H0.
+  apply In_app_imp_In_app.
+  apply mlSortOfFormRelIn; now auto.
+  apply In_app_imp_In_app.
+  apply mlSortOfFormRelIn; now auto.
+  apply mlSortOfRelUsingArityIn; now auto.
+Qed.
+
+Lemma mlSortOfRelArityIn: forall m r s,
+  In (MLR r) (mlModelIds m) -> In s (mlRelArity r) -> In (MLS s) (mlModelIds m).
+Proof.
+  unfold mlModelIds; intros.
+  revert H.
+  apply utils.In_app_imp_In_app.
+  apply In_cmap_In_cmap.
+  intro; apply mlSortOfFormRelIn; now auto.
+  
+  apply utils.In_app_imp_In_app.
+  apply In_cmap_In_cmap.
+  intro; apply mlSortOfEvtArityIn;  now auto.
+
+  apply utils.In_app_imp_In_app.
+  apply In_cmap_In_cmap.
+  intro; apply mlSortOfPathArityIn; now auto.
+  apply mlSortOfRelChkArityIn; now auto.
+Qed.
+
+Lemma mlSortOfVarsIn: forall m v,
+  In v (mlAllVariables m) -> In (mlVarSort v) (mlSorts m).
+Proof.
+  intros.
+  unfold mlAllVariables in H; unfold mlSorts.
+  apply imap_filiter_in_elim in H.
+  destruct H as [u [h1 [h2 h3]]]; subst v.
+  destruct u; simpl in *; try tauto.
+  apply (imap_filter_In_intro _ _ isMLSortDec (mlModelIds m)
+    (fun (v0 : mlIdent) (h0 : isMLSort v0) (_ : In v0 (mlModelIds m))
+      => getMLSort v0 h0) (MLS (mlVarSort v)) I).
+  apply mlSortOfVarIn; auto.
+Qed.
+
+Lemma mlSortOfCstsIn: forall m c,
+  In c (mlAllConstants m) -> In (mlCstSort c) (mlSorts m).
+Proof.
+  intros.
+  unfold mlAllConstants in H; unfold mlSorts.
+  apply imap_filiter_in_elim in H.
+  destruct H as [u [h1 [h2 h3]]]; subst c.
+  destruct u; simpl in *; try tauto.
+  apply (imap_filter_In_intro _ _ isMLSortDec (mlModelIds m)
+    (fun (v0 : mlIdent) (h0 : isMLSort v0) (_ : In v0 (mlModelIds m))
+      => getMLSort v0 h0) (MLS (mlCstSort c)) I).
+  apply mlSortOfCstIn; auto.
+Qed.
+
+Lemma mlSortOfRelAritiesIn: forall m r,
+  In r (mlRelations m) -> forall s, In s (mlRelArity r) -> In s (mlSorts m).
+Proof.
+  intros.
+  unfold mlRelations in H; unfold mlSorts.
+  apply imap_filiter_in_elim in H.
+  destruct H as [u [h1 [h2 h3]]]; subst r.
+  destruct u; simpl in *; try tauto.
+  apply (imap_filter_In_intro _ _ isMLSortDec (mlModelIds m)
+    (fun (v0 : mlIdent) (h0 : isMLSort v0) (_ : In v0 (mlModelIds m))
+      => getMLSort v0 h0) (MLS s) I).
+  revert H0; apply mlSortOfRelArityIn; auto.
+Qed.
+
